src/coq/Utils/Monads.v
@@ -16,3 +16,14 @@ Fixpoint foldM {a b} {M} `{Monad M} (f : b -> a -> M b ) (acc : b) (l : list a) 
        b <- f acc x;;
        foldM f b xs
      end.
+
+Lemma map_monad_In {m : Type -> Type} {H : Monad m} {A B} (l : list A) (f: forall (x : A), In x l -> m B) : m (list B).
+Proof.
+  induction l.
+  - exact (ret []).
+  - refine (b <- f a _;; bs <- IHl _;; ret (b::bs)).
+    + cbn; auto.
+    + intros x Hin.
+      apply (f x).
+      cbn; auto.
+Defined.
